Rename Big and Small cases

thys/Real_Time_Deque/Big.thy
@@ -6,17 +6,17 @@ begin
 
 text \<open>\<^noindent> The bigger end of the deque during rebalancing can be in two phases:
 
- \<^descr> \<open>Reverse\<close>: Using the \<open>step\<close> function the originally contained elements, 
+ \<^descr> \<open>Big1\<close>: Using the \<open>step\<close> function the originally contained elements, 
     which will be kept in this end, are reversed.
- \<^descr> \<open>Common\<close>: Specified in theory \<open>Common\<close>. Is used to reverse the elements from the previous phase 
+ \<^descr> \<open>Big2\<close>: Specified in theory \<open>Common\<close>. Is used to reverse the elements from the previous phase 
     again to get them in the original order.
 
 \<^noindent> Each phase contains a \<open>current\<close> state, which holds the original elements of the deque end. 
 \<close>
 
 datatype (plugins del: size) 'a big_state = 
-     Reverse "'a current" "'a stack" "'a list" nat
-   | Common "'a common_state"
+     Big1 "'a current" "'a stack" "'a list" nat
+   | Big2 "'a common_state"
 
 text \<open>\<^noindent> Functions:
 
@@ -27,21 +27,21 @@ instantiation big_state ::(type) step
 begin
 
 fun step_big_state :: "'a big_state \<Rightarrow> 'a big_state" where
-  "step (Common state) = Common (step state)"
-| "step (Reverse current _ aux 0) = Common (normalize (Copy current aux [] 0))"
-| "step (Reverse current big aux count) = 
-     Reverse current (Stack.pop big) ((Stack.first big)#aux) (count - 1)"
+  "step (Big2 state) = Big2 (step state)"
+| "step (Big1 current _ aux 0) = Big2 (normalize (Copy current aux [] 0))"
+| "step (Big1 current big aux count) = 
+     Big1 current (Stack.pop big) ((Stack.first big)#aux) (count - 1)"
 
 instance..
 end
 
 fun push :: "'a \<Rightarrow> 'a big_state \<Rightarrow> 'a big_state" where
-  "push x (Common state) = Common (Common.push x state)"
-| "push x (Reverse current big aux count) = Reverse (Current.push x current) big aux count"
+  "push x (Big2 state) = Big2 (Common.push x state)"
+| "push x (Big1 current big aux count) = Big1 (Current.push x current) big aux count"
 
 fun pop :: "'a big_state \<Rightarrow> 'a * 'a big_state" where
-  "pop (Common state) = (let (x, state) = Common.pop state in (x, Common state))"
-| "pop (Reverse current big aux count) = 
-    (first current, Reverse (drop_first current) big aux count)"
+  "pop (Big2 state) = (let (x, state) = Common.pop state in (x, Big2 state))"
+| "pop (Big1 current big aux count) = 
+    (first current, Big1 (drop_first current) big aux count)"
 
 end
