thys/Real_Time_Deque/Big_Aux.thy
@@ -11,22 +11,22 @@ text \<open>\<^noindent> Functions:
 \<^descr> \<open>list_current\<close>: List abstraction of the elements currently in this deque end.\<close>
 
 fun list :: "'a big_state \<Rightarrow> 'a list" where
-  "list (Common common) = Common_Aux.list common"
-| "list (Reverse (Current extra _ _ remained) big aux count) = (
+  "list (Big2 common) = Common_Aux.list common"
+| "list (Big1 (Current extra _ _ remained) big aux count) = (
    let reversed = take_rev count (Stack_Aux.list big) @ aux in
     extra @ (take_rev remained reversed)
   )"
 
 fun list_current :: "'a big_state \<Rightarrow> 'a list" where
-  "list_current (Common common) = Common_Aux.list_current common"
-| "list_current (Reverse current _ _ _) = Current_Aux.list current"
+  "list_current (Big2 common) = Common_Aux.list_current common"
+| "list_current (Big1 current _ _ _) = Current_Aux.list current"
 
 instantiation big_state ::(type) invar
 begin
 
 fun invar_big_state :: "'a big_state \<Rightarrow> bool" where
-  "invar (Common state) \<longleftrightarrow> invar state"
-| "invar (Reverse current big aux count) \<longleftrightarrow> (
+  "invar (Big2 state) \<longleftrightarrow> invar state"
+| "invar (Big1 current big aux count) \<longleftrightarrow> (
    case current of Current extra added old remained \<Rightarrow>
       invar current
     \<and> List.length aux \<ge> remained - count
@@ -44,8 +44,8 @@ instantiation big_state ::(type) size
 begin
 
 fun size_big_state :: "'a big_state \<Rightarrow> nat" where
-  "size (Common state) = size state"
-| "size (Reverse current _ _ _) = min (size current) (size_new current)"
+  "size (Big2 state) = size state"
+| "size (Big1 current _ _ _) = min (size current) (size_new current)"
 
 instance..
 end
@@ -54,8 +54,8 @@ instantiation big_state ::(type) size_new
 begin
 
 fun size_new_big_state :: "'a big_state \<Rightarrow> nat" where
-  "size_new (Common state) = size_new state"
-| "size_new (Reverse current _ _ _) = size_new current"
+  "size_new (Big2 state) = size_new state"
+| "size_new (Big1 current _ _ _) = size_new current"
 
 instance..
 end
@@ -64,8 +64,8 @@ instantiation big_state ::(type) remaining_steps
 begin
 
 fun remaining_steps_big_state :: "'a big_state \<Rightarrow> nat" where
-  "remaining_steps (Common state) = remaining_steps state"
-| "remaining_steps (Reverse (Current _ _ _ remaining) _ _ count) = count + remaining + 1"
+  "remaining_steps (Big2 state) = remaining_steps state"
+| "remaining_steps (Big1 (Current _ _ _ remaining) _ _ count) = count + remaining + 1"
 
 instance..
 end
