thys/Real_Time_Deque/Small.thy
@@ -7,17 +7,17 @@ begin
 text \<open>
 \<^noindent> The smaller end of the deque during \<open>Rebalancing\<close> can be in one three phases:
 
- \<^descr> \<open>Reverse1\<close>: Using the \<open>step\<close> function the originally contained elements are reversed.
- \<^descr> \<open>Reverse2\<close>: Using the \<open>step\<close> function the newly obtained elements from the bigger end are reversed on top of the ones reversed in the previous phase.
- \<^descr> \<open>Common\<close>: See theory \<open>Common\<close>. Is used to reverse the elements from the two previous phases again to get them again in the original order.
+ \<^descr> \<open>Small1\<close>: Using the \<open>step\<close> function the originally contained elements are reversed.
+ \<^descr> \<open>Small2\<close>: Using the \<open>step\<close> function the newly obtained elements from the bigger end are reversed on top of the ones reversed in the previous phase.
+ \<^descr> \<open>Small3\<close>: See theory \<open>Common\<close>. Is used to reverse the elements from the two previous phases again to get them again in the original order.
 
 \<^noindent> Each phase contains a \<open>current\<close> state, which holds the original elements of the deque end. 
 \<close>
 
 datatype (plugins del: size) 'a small_state =
-   Reverse1 "'a current" "'a stack" "'a list"
- | Reverse2 "'a current" "'a list" "'a stack" "'a list" nat
- | Common "'a common_state"
+   Small1 "'a current" "'a stack" "'a list"
+ | Small2 "'a current" "'a list" "'a stack" "'a list" nat
+ | Small3 "'a common_state"
 
 text \<open>\<^noindent> Functions:
 
@@ -28,35 +28,35 @@ instantiation small_state::(type) step
 begin
 
 fun step_small_state :: "'a small_state \<Rightarrow> 'a small_state" where
-  "step (Common state) = Common (step state)"
-| "step (Reverse1 current small auxS) = (
+  "step (Small3 state) = Small3 (step state)"
+| "step (Small1 current small auxS) = (
     if is_empty small 
-    then Reverse1 current small auxS 
-    else Reverse1 current (Stack.pop small) ((Stack.first small)#auxS)
+    then Small1 current small auxS 
+    else Small1 current (Stack.pop small) ((Stack.first small)#auxS)
   )"
-| "step (Reverse2 current auxS big newS count) = (
+| "step (Small2 current auxS big newS count) = (
     if is_empty big
-    then Common (normalize (Copy current auxS newS count))
-    else Reverse2 current auxS (Stack.pop big) ((Stack.first big)#newS) (count + 1)
+    then Small3 (normalize (Copy current auxS newS count))
+    else Small2 current auxS (Stack.pop big) ((Stack.first big)#newS) (count + 1)
   )"
 
 instance..
 end
 
 fun push :: "'a \<Rightarrow> 'a small_state \<Rightarrow> 'a small_state" where
-  "push x (Common state) = Common (Common.push x state)"
-| "push x (Reverse1 current small auxS) = Reverse1 (Current.push x current) small auxS"
-| "push x (Reverse2 current auxS big newS count) = 
-    Reverse2 (Current.push x current) auxS big newS count"
+  "push x (Small3 state) = Small3 (Common.push x state)"
+| "push x (Small1 current small auxS) = Small1 (Current.push x current) small auxS"
+| "push x (Small2 current auxS big newS count) = 
+    Small2 (Current.push x current) auxS big newS count"
 
 fun pop :: "'a small_state \<Rightarrow> 'a * 'a small_state" where
-  "pop (Common state) = (
+  "pop (Small3 state) = (
     let (x, state) = Common.pop state 
-    in (x, Common state)
+    in (x, Small3 state)
   )"
-| "pop (Reverse1 current small auxS) = 
-    (first current, Reverse1 (drop_first current) small auxS)"
-| "pop (Reverse2 current auxS big newS count) = 
-    (first current, Reverse2 (drop_first current) auxS big newS count)"
+| "pop (Small1 current small auxS) = 
+    (first current, Small1 (drop_first current) small auxS)"
+| "pop (Small2 current auxS big newS count) = 
+    (first current, Small2 (drop_first current) auxS big newS count)"
 
 end
