thys/Real_Time_Deque/Small_Aux.thy
@@ -9,21 +9,21 @@ text \<open>\<^noindent> Functions:
  \<^descr> \<open>list_current\<close>: List abstraction of the elements currently in this deque end.\<close>
 
 fun list :: "'a small_state \<Rightarrow> 'a list" where
-  "list (Common common) = Common_Aux.list common"
-| "list (Reverse2 (Current extra _ _ remained) aux big new count) =
+  "list (Small3 common) = Common_Aux.list common"
+| "list (Small2 (Current extra _ _ remained) aux big new count) =
   extra @ (take_rev (remained - (count + size big)) aux) @ (rev (Stack_Aux.list big) @ new)"
 
 fun list_current :: "'a small_state \<Rightarrow> 'a list" where
-  "list_current (Common common) = Common_Aux.list_current common"
-| "list_current (Reverse2 current _ _ _ _) = Current_Aux.list current"
-| "list_current (Reverse1 current _ _) = Current_Aux.list current"
+  "list_current (Small3 common) = Common_Aux.list_current common"
+| "list_current (Small2 current _ _ _ _) = Current_Aux.list current"
+| "list_current (Small1 current _ _) = Current_Aux.list current"
 
 instantiation small_state::(type) invar
 begin
 
 fun invar_small_state :: "'a small_state \<Rightarrow> bool" where
-  "invar (Common state) = invar state"
-| "invar (Reverse2 current auxS big newS count) = (
+  "invar (Small3 state) = invar state"
+| "invar (Small2 current auxS big newS count) = (
    case current of Current _ _ old remained \<Rightarrow>
       remained = count + size big + size old
     \<and> count = List.length newS
@@ -31,7 +31,7 @@ fun invar_small_state :: "'a small_state \<Rightarrow> bool" where
     \<and> List.length auxS \<ge> size old
     \<and> Stack_Aux.list old = rev (take (size old) auxS)
   )"
-| "invar (Reverse1 current small auxS) = (
+| "invar (Small1 current small auxS) = (
    case current of Current _ _ old remained \<Rightarrow>
       invar current
     \<and> remained \<ge> size old
@@ -46,9 +46,9 @@ instantiation small_state::(type) size
 begin
 
 fun size_small_state :: "'a small_state \<Rightarrow> nat" where
-  "size (Common state) = size state"
-| "size (Reverse2 current _ _ _ _) = min (size current) (size_new current)"
-| "size (Reverse1 current _ _) = min (size current) (size_new current)"
+  "size (Small3 state) = size state"
+| "size (Small2 current _ _ _ _) = min (size current) (size_new current)"
+| "size (Small1 current _ _) = min (size current) (size_new current)"
 
 instance..
 end
@@ -57,9 +57,9 @@ instantiation small_state::(type) size_new
 begin
 
 fun size_new_small_state :: "'a small_state \<Rightarrow> nat" where
-  "size_new (Common state) = size_new state"
-| "size_new (Reverse2 current _ _ _ _) = size_new current"
-| "size_new (Reverse1 current _ _) = size_new current"
+  "size_new (Small3 state) = size_new state"
+| "size_new (Small2 current _ _ _ _) = size_new current"
+| "size_new (Small1 current _ _) = size_new current"
 
 instance..
 end
